Complexitylib/Models.lean
@@ -3,3 +3,11 @@ import Complexitylib.Models.TuringMachine.Internal
 import Complexitylib.Models.TuringMachine.Combinators
 import Complexitylib.Models.TuringMachine.Combinators.Internal
 import Complexitylib.Models.TuringMachine.Combinators.ComplementInternal
+import Complexitylib.Models.TuringMachine.Combinators.SeqInternal
+import Complexitylib.Models.TuringMachine.Combinators.IfInternal
+import Complexitylib.Models.TuringMachine.Combinators.LoopInternal
+import Complexitylib.Models.TuringMachine.Hoare
+import Complexitylib.Models.TuringMachine.UTM.Defs
+import Complexitylib.Models.TuringMachine.UTM.Helpers
+import Complexitylib.Models.TuringMachine.UTM.HelpersInternal
+import Complexitylib.Models.TuringMachine.UTM.SimStep
